---
title: Testing
date: 2023-07-27
categories: [Math]
tags: [blog]
math: true
---
This is my first post.

As an introduction, here is a math problem I really enjoyed solving.

<b>Problem</b>

Let $P_{n} (x)$ be the $n$-th Chebyshev polynomial. 

Prove that

$$P_{n} (x)-1=2^{n-1}\prod_{k=1}^n \left(x-\cos\left(\frac{2\pi k}{n}\right)\right)$$

<b>Solution</b>

<blockquote style="color: #1e2f97; border-left-color: #1e2f97">
<b>Definition</b> $$P_{n}(x)=\frac{1}{2}\left(x+\sqrt{x^2-1}\right)^n+\frac{1}{2}\left(x-\sqrt{x^2-1}\right)^n$$
</blockquote>

So it suffices to prove,

$$\frac{1}{2}\left(x+\sqrt{x^2-1}\right)^n+\frac{1}{2}\left(x-\sqrt{x^2-1}\right)^n-1=2^{n-1}\prod_{k=1}^n \left(x-\cos\left(\frac{2\pi k}{n}\right)\right)$$

Note the $LHS$ can be rewritten as,

$$\frac{1}{2}\left(x+\sqrt{x^2-1}\right)^n+\frac{1}{2}\left(x-\sqrt{x^2-1}\right)^n-\left(1\right)^n$$

Since this is a linear recurrence with order of $3$, if $n=1,2,3$ works, we are done.

<blockquote style="color: #357a38; border-left-color: #357a38">
<b>Case:</b> $n=1$
</blockquote>

$$\frac{1}{2}\left(x+\sqrt{x^2-1}\right)+\frac{1}{2}\left(x-\sqrt{x^2-1}\right)-1=2^{0}\prod_{k=1}^1\left(x-\cos\left(\frac{2\pi k}{1}\right)\right)$$
    
Simplifying gives,
    
$$x-1=1\left(x-\cos\left(2\pi\right)\right)$$
    
This indeed works.
 
 <blockquote style="color: #357a38; border-left-color: #357a38">
<b>Case:</b> $n=2$
</blockquote>

$$\frac{1}{2}\left(x+\sqrt{x^2-1}\right)^2+\frac{1}{2}\left(x-\sqrt{x^2-1}\right)^2-1=2^{1}\prod_{k=1}^2\left(x-\cos\left(\frac{2\pi k}{2}\right)\right)$$

Simplifying gives,

$$2x^2-2=2(x-(-1))(x-1)\rightarrow 2x^2-2=2x^2-2$$

This also works.
 
<blockquote style="color: #357a38; border-left-color: #357a38">
<b>Case:</b> $n=3$
</blockquote>

$$\frac{1}{2}\left(x+\sqrt{x^2-1}\right)^3+\frac{1}{2}\left(x-\sqrt{x^2-1}\right)^3-1=2^{2}\prod_{k=1}^3\left(x-\cos\left(\frac{2\pi k}{3}\right)\right)$$

Simplifying gives,

$$4x^3-3x-1=4\left(x-\left(-\frac{1}{2}\right)\right)\left(x-\left(-\frac{1}{2}\right)\right)\left(x-1\right)$$

The $RHS$ simplifies to $$(4x^2+4x+1)(x-1)=4x^3-3x-1$$ which is indeed the $LHS$.

Hence, we are done.
